more

Weidenbach_Book/Array_Array_List.thy
@@ -7,6 +7,33 @@ fun heap_list_all :: "('a \<Rightarrow> 'b \<Rightarrow> assn) \<Rightarrow> 'a 
 | \<open>heap_list_all R (x # xs) (y # ys) = R x y * heap_list_all R xs ys\<close>
 | \<open>heap_list_all R _ _ = false\<close>
 
+definition heap_list_all_nth:: "('a \<Rightarrow> 'b \<Rightarrow> assn) \<Rightarrow> nat list \<Rightarrow>  'a list \<Rightarrow> 'b list \<Rightarrow> assn" where
+  \<open>heap_list_all_nth R is xs ys = foldr (op *) (map (\<lambda>i. R (xs ! i) (ys ! i)) is) emp\<close>
+
+lemma heap_list_all_nth_emty[simp]: \<open>heap_list_all_nth R [] [] [] = emp\<close>
+  unfolding heap_list_all_nth_def by auto
+
+lemma heap_list_all_heap_list_all_nth:
+  \<open>length xs = length ys \<Longrightarrow> heap_list_all R xs ys = heap_list_all_nth R [0..< length xs] xs ys\<close>
+proof (induction R xs ys rule: heap_list_all.induct)
+  case (2 R x xs y ys) note IH = this
+  then have IH: \<open>heap_list_all R xs ys = heap_list_all_nth R [0..<length xs] xs ys\<close>
+    by auto
+  have upt: \<open>[0..<length (x # xs)] = 0 # [1..<Suc (length xs)]\<close>
+    by (simp add: upt_rec)
+  have upt_map_Suc: \<open>[1..<Suc (length xs)] = map Suc [0..<length xs]\<close>
+    by (induction xs) auto
+  have map: \<open>(map (\<lambda>i. R ((x # xs) ! i) ((y # ys) ! i)) [1..<Suc (length xs)]) =
+    (map (\<lambda>i. R (xs ! i) (ys ! i)) [0..< (length xs)])\<close>
+    unfolding upt_map_Suc map_map by auto
+  have 1: \<open>heap_list_all_nth R [0..<length (x # xs)] (x # xs) (y # ys) =
+    R x y * heap_list_all_nth R [0..<length xs] xs ys\<close>
+    unfolding heap_list_all_nth_def upt
+    by (simp only: list.map foldr.simps map) auto
+  show ?case
+    using IH unfolding 1 by auto
+qed auto
+
 definition arrayO:: \<open>('a \<Rightarrow> 'b::heap \<Rightarrow> assn) \<Rightarrow> 'a list \<Rightarrow> 'b array \<Rightarrow> assn\<close> where
   \<open>arrayO R' xs axs \<equiv> \<exists>\<^sub>A p. array_assn id_assn p axs * heap_list_all R' xs p\<close>
 
@@ -81,7 +108,7 @@ proof -
       by (auto simp: run.simps tap_def arrayO_def execute_simps
           mod_star_conv array_assn_def is_array_def nth_aa_def Array.nth_def
           Abs_assn_inverse heap_list_add_same_length snga_assn_def
-          execute_bind_case arl_get_def split_beta
+           arl_get_def split_beta
           split: option.splits)
     have ex: \<open>execute (nth_aa ai i j) h = Some (Array.get h (fst (Array.get h ai ! i)) ! j, h)\<close>
       using run h assms i_le
@@ -128,12 +155,90 @@ term \<open>Array.set a (list_update (Array.get h a) i x) h\<close>
 term arl_assn
 term arl_append
 
-definition append_el_aa where
+definition append_el_aa :: "('a::{default,heap} array_list) array \<Rightarrow>
+  nat \<Rightarrow> 'a \<Rightarrow> ('a array_list) array Heap"where
 "append_el_aa \<equiv> \<lambda>a i x. do {
   j \<leftarrow> Array.nth a i;
   a' \<leftarrow> arl_append j x;
   Array.upd i a' a
   }"
+definition append_ll :: "'a list list \<Rightarrow> nat \<Rightarrow> 'a \<Rightarrow> 'a list list" where
+  \<open>append_ll xs i x = list_update xs i (xs ! i @ [x])\<close>
+(* src si dst di (Suc l) *)
+lemma
+  \<open>i < Array.length h aa \<Longrightarrow> execute (blit aa i dst i l) h \<noteq> None\<close>
+  apply (induction l)
+   apply (auto simp: execute_simps execute_bind_case Array.nth_def
+      Array.upd_def
+      split: option.splits)
+    oops
+lemma nth_aa_hnr[sepref_fr_rules]:
+  fixes R ::  \<open>'a \<Rightarrow> 'b :: {heap, default}\<Rightarrow> assn\<close>
+  assumes p: \<open>is_pure R\<close>
+  shows
+    \<open>(uncurry2 append_el_aa, uncurry2 (RETURN \<circ>\<circ>\<circ> append_ll)) \<in>
+     [\<lambda>((l,i),x). i < length l]\<^sub>a (arrayO (arl_assn R))\<^sup>d *\<^sub>a nat_assn\<^sup>k *\<^sub>a R\<^sup>k \<rightarrow> (arrayO (arl_assn R))\<close>
+proof -
+  obtain R' where R: \<open>the_pure R = R'\<close> and R': \<open>R = pure R'\<close>
+    using p by fastforce
+  have [simp]: \<open>(\<exists>\<^sub>Ax. arrayO (arl_assn R) a ai * R x r * true * \<up> (x = a ! ba ! b)) =
+     (arrayO (arl_assn R) a ai * R (a ! ba ! b) r * true)\<close> for a ai ba b r
+    by (auto simp: ex_assn_def)
+  have ?thesis
+    apply sepref_to_hoare
+    apply (auto simp: append_el_aa_def (* arrayO_def *) array_assn_def is_array_def)
+    apply (rule bind_rule)
+      -- \<open>some work on ArrayO missing\<close>
+      sorry
+    show ?thesis
+  proof (sepref_to_hoare, clarsimp simp only: hoare_triple_def Let_def, intro allI impI conjI)
+    fix a :: \<open>'a list list\<close> and ai :: \<open>('b array_list) array\<close> and
+      h :: Heap.heap and as:: \<open>nat set\<close> and \<sigma> :: \<open>Heap.heap option\<close> and r :: \<open>('b array_list) array\<close> and
+      i i' :: nat and x' :: 'a and x :: 'b
+    assume
+      i: \<open>i < length a\<close> and
+      h: \<open>(h, as) \<Turnstile> R x' x * \<up> ((i', i) \<in> nat_rel) * arrayO (arl_assn R) a ai\<close> and
+      run: \<open>run (append_el_aa ai i' x) (Some h) \<sigma> r\<close>
+    have i'_i[simp]: \<open>i' = i\<close>
+      using h by auto
+    have i_le: \<open>i < Array.length h ai\<close>
+      using h i unfolding arrayO_def array_assn_def is_array_def
+      by (auto simp: run.simps tap_def arrayO_def
+          mod_star_conv array_assn_def is_array_def
+          Abs_assn_inverse heap_list_add_same_length length_def snga_assn_def)
+    have xs_i: \<open>\<exists>as'. (h, as') \<Turnstile> (arl_assn R) (a ! i) (Array.get h ai ! i)\<close>
+      using h i unfolding arrayO_def array_assn_def is_array_def
+      using models_heap_list_all_models_nth[of _ _ _ _ _ i]
+      by (auto simp: run.simps tap_def arrayO_def
+          mod_star_conv array_assn_def is_array_def
+          Abs_assn_inverse heap_list_add_same_length length_def snga_assn_def)
+    have ex_arl: \<open>execute (arl_append (Array.get h ai ! i) x) h \<noteq> None\<close>
+      using run h assms i_le i xs_i
+      using arl_append_rule[of _ \<open>Array.get h ai ! i\<close> x, unfolded hoare_triple_def]
+      unfolding arl_assn_def hr_comp_def
+(*       apply (cases \<open>Array.get h ai ! i\<close>)
+      apply (auto simp: run.simps tap_def arrayO_def execute_simps arl_append_def
+          mod_star_conv array_assn_def is_array_def append_el_aa_def Array.nth_def
+          Abs_assn_inverse heap_list_add_same_length length_def snga_assn_def
+          array_grow_def Let_def split_beta
+          execute_bind_case split: option.splits if_splits) *)
+
+
+
+
+
+    have ex: \<open>execute (append_el_aa ai i x) h = Some x'''\<close>
+      using run h assms i_le
+      apply (auto simp: run.simps tap_def arrayO_def execute_simps
+          mod_star_conv array_assn_def is_array_def append_el_aa_def Array.nth_def
+          Abs_assn_inverse heap_list_add_same_length length_def snga_assn_def
+          execute_bind_case split: option.splits)
+        oops
+    show \<open>\<not> is_exn \<sigma>\<close>
+      using run h assms
+      by (auto simp: run.simps tap_def arrayO_def execute_simps
+          mod_star_conv array_assn_def is_array_def Array.nth_def
+          Abs_assn_inverse heap_list_add_same_length length_def snga_assn_def)
 
 
 
